Makefile
@@ -6,5 +6,5 @@ verify:
 compile: 
 	{ \
 	dotnet build smt_interface/csharp_smt_interface ;\
-	dafny /noVerify /out:smt_interface/csharp_smt_interface/bin/Debug/net6.0/AllTransformations.dll /compile:2 /spillTargetCode:3 /useRuntimeLib transformations/AllTransformations.dfy util/Shims.cs smt_interface/csharp_smt_interface/bin/Debug/net6.0/csharp_smt_interface.dll smt_interface/csharp_smt_interface/bin/Debug/net6.0/Boogie.VCExpr.dll ;\
+	dafny /noVerify /out:smt_interface/csharp_smt_interface/bin/Debug/net6.0/BoogieV.dll /compile:2 /spillTargetCode:3 /useRuntimeLib transformations/AllTransformations.dfy util/Shims.cs smt_interface/csharp_smt_interface/bin/Debug/net6.0/csharp_smt_interface.dll smt_interface/csharp_smt_interface/bin/Debug/net6.0/Boogie.VCExpr.dll ;\
 	}
