lang/README.md
@@ -1,0 +1,12 @@
+# Formalization of BoogieV
+
+## Most important files
+* `BoogieLang.dfy`: AST for BoogieV (expressions, commands)
+* `BoogieSemantics.dfy`: Semantics for BoogieV using weakest preconditions
+* `Cfg.dfy`: Representation for control-flow graphs (CFGs) and a semantics for acyclic
+CFGs based on weakest preconditions
+
+## Boogie semantics main definitions
+The Boogie semantics is defined via the `WpCmd` function in `BoogieSemantics.dfy`
+that defines the weakest precondition for commands, which relies on the 
+evaluation of expressions `EvalExpr` function.
